Added completeness theorem

IMP-/IMP_Calls.thy
@@ -2,6 +2,8 @@
 
 theory IMP_Calls imports Vars begin
 
+section "IMP"
+
 text \<open>IMP with calls to IMP- programs (explicitly stored).\<close>
 datatype
   com' = SKIP'
@@ -32,18 +34,17 @@ unbundle com'_syntax
 inductive
   big_step_t' :: "com' \<times> state \<Rightarrow> nat \<Rightarrow> state \<Rightarrow> bool"  ("_ \<Rightarrow>''\<^bsup> _ \<^esup> _" 55)
 where
-Skip: "(SKIP',s) \<Rightarrow>'\<^bsup> Suc (0::nat) \<^esup> s"|
-Assign: "(x ::= a,s) \<Rightarrow>'\<^bsup> Suc (Suc 0) \<^esup> s(x := aval a s)" |
-Seq: "\<lbrakk> (c1,s1) \<Rightarrow>'\<^bsup> x \<^esup> s2;  (c2,s2) \<Rightarrow>'\<^bsup> y \<^esup> s3 ; z=x+y \<rbrakk> \<Longrightarrow> (c1;;c2, s1) \<Rightarrow>'\<^bsup> z \<^esup> s3" |
-IfTrue: "\<lbrakk> s b \<noteq> 0;  (c1,s) \<Rightarrow>'\<^bsup> x \<^esup> t; y=x+1 \<rbrakk> \<Longrightarrow> (IF b \<noteq>0 THEN c1 ELSE c2, s) \<Rightarrow>'\<^bsup> y \<^esup> t" |
-IfFalse: "\<lbrakk> s b = 0; (c2,s) \<Rightarrow>'\<^bsup> x \<^esup> t; y=x+1  \<rbrakk> \<Longrightarrow> (IF b \<noteq>0 THEN c1 ELSE c2, s) \<Rightarrow>'\<^bsup> y \<^esup> t" |
-WhileFalse: "\<lbrakk> s b = 0 \<rbrakk> \<Longrightarrow> (WHILE b \<noteq>0 DO c,s) \<Rightarrow>'\<^bsup> Suc (Suc 0) \<^esup> s" |
-WhileTrue: "\<lbrakk> s1 b \<noteq> 0;  (c,s1) \<Rightarrow>'\<^bsup> x \<^esup> s2;  (WHILE b \<noteq>0 DO c, s2) \<Rightarrow>'\<^bsup> y \<^esup> s3; 1+x+y=z  \<rbrakk> 
+Skip': "(SKIP',s) \<Rightarrow>'\<^bsup> Suc (0::nat) \<^esup> s"|
+Assign': "(x ::= a,s) \<Rightarrow>'\<^bsup> Suc (Suc 0) \<^esup> s(x := aval a s)" |
+Seq': "\<lbrakk> (c1,s1) \<Rightarrow>'\<^bsup> x \<^esup> s2;  (c2,s2) \<Rightarrow>'\<^bsup> y \<^esup> s3 ; z=x+y \<rbrakk> \<Longrightarrow> (c1;;c2, s1) \<Rightarrow>'\<^bsup> z \<^esup> s3" |
+IfTrue': "\<lbrakk> s b \<noteq> 0;  (c1,s) \<Rightarrow>'\<^bsup> x \<^esup> t; y=x+1 \<rbrakk> \<Longrightarrow> (IF b \<noteq>0 THEN c1 ELSE c2, s) \<Rightarrow>'\<^bsup> y \<^esup> t" |
+IfFalse': "\<lbrakk> s b = 0; (c2,s) \<Rightarrow>'\<^bsup> x \<^esup> t; y=x+1  \<rbrakk> \<Longrightarrow> (IF b \<noteq>0 THEN c1 ELSE c2, s) \<Rightarrow>'\<^bsup> y \<^esup> t" |
+WhileFalse': "\<lbrakk> s b = 0 \<rbrakk> \<Longrightarrow> (WHILE b \<noteq>0 DO c,s) \<Rightarrow>'\<^bsup> Suc (Suc 0) \<^esup> s" |
+WhileTrue': "\<lbrakk> s1 b \<noteq> 0;  (c,s1) \<Rightarrow>'\<^bsup> x \<^esup> s2;  (WHILE b \<noteq>0 DO c, s2) \<Rightarrow>'\<^bsup> y \<^esup> s3; 1+x+y=z  \<rbrakk> 
     \<Longrightarrow> (WHILE b \<noteq>0 DO c, s1) \<Rightarrow>'\<^bsup> z \<^esup> s3" |
 \<comment> \<open>The only change: The called program is executed on a state that agrees on all the variables in
     the subprogram. In the caller, only the result variable is affected.\<close>
-Call: "\<lbrakk> (c,s') \<Rightarrow>\<^bsup> z \<^esup> t; s' = s on set (r#vars c) \<rbrakk>
-    \<Longrightarrow> (CALL c RETURN r,s) \<Rightarrow>'\<^bsup> z \<^esup> (s(r:=t r))"
+Call': "(c,s) \<Rightarrow>\<^bsup> z \<^esup> t \<Longrightarrow> (CALL c RETURN r,s) \<Rightarrow>'\<^bsup> z \<^esup> (s(r:=t r))"
 
 text \<open>For compilation to IMP-, skip to final proof.\<close>
 
@@ -58,6 +59,7 @@ inductive_cases Assign'_tE[elim!]: "(x ::= a,s) \<Rightarrow>'\<^bsup> p \<^esup
 inductive_cases Seq'_tE[elim!]: "(c1;;c2,s1) \<Rightarrow>'\<^bsup> p \<^esup> s3"
 inductive_cases If'_tE[elim!]: "(IF b \<noteq>0 THEN c1 ELSE c2,s) \<Rightarrow>'\<^bsup> x \<^esup> t"
 inductive_cases Call'_tE[elim!]: " (CALL c RETURN v,s) \<Rightarrow>'\<^bsup> z \<^esup> t"
+thm Call'_tE
 inductive_cases While'_tE[elim]: "(WHILE b \<noteq>0 DO c,s) \<Rightarrow>'\<^bsup> x \<^esup> t"
 lemma Seq'': "\<lbrakk> (c1,s1) \<Rightarrow>'\<^bsup> x \<^esup> s2;  (c2,s2) \<Rightarrow>'\<^bsup> y \<^esup> s3  \<rbrakk> \<Longrightarrow> (c1;;c2, s1) \<Rightarrow>'\<^bsup> x + y \<^esup> s3"
   by auto
@@ -76,6 +78,10 @@ fun vars_com' :: "com' \<Rightarrow> vname list" where
 instance ..
 
 end
+
+section "Inlining"
+
+subsection "Memory mapping"
 
 definition fresh :: "vname list \<Rightarrow> vname \<Rightarrow> vname" where 
   "fresh S v = CHR ''.'' # concat S @ v"
@@ -117,94 +123,102 @@ lemma rvars_ssubst[simp]: "rvars (ssubst m vs) = m ` set vs"
 lemma ssubst_unchanged: "(ssubst m vs,s) \<Rightarrow>\<^bsup>z\<^esup> t \<Longrightarrow> (\<forall>v\<in>set vs. m v \<notin> set vs) \<Longrightarrow> s = t on set vs"
   apply auto
   by (metis (mono_tags, opaque_lifting) image_iff rvars_ssubst rvars_unchanged)
-  
-lemma ssubst_sound:
-  "\<lbrakk>(ssubst m vs,s) \<Rightarrow>\<^bsup>z\<^esup> t; inj_on m (set vs); (\<forall>v\<in>set vs. m v \<notin> set vs)\<rbrakk> \<Longrightarrow> 
-s = t o m on set vs \<and> z = Suc (2 * length vs)"
-proof (induction vs arbitrary: z s t )
+
+lemma ssubst_correct:
+  "\<lbrakk> inj_on m (set vs); (\<forall>v\<in>set vs. m v \<notin> set vs) \<rbrakk>
+    \<Longrightarrow> \<exists>t. (ssubst m vs,s) \<Rightarrow>\<^bsup>Suc (2 * length vs)\<^esup> t \<and> s = t o m on set vs"
+proof (induction vs arbitrary: s)
   case (Cons v vs)
-  hence "((m v) ::= A (V v) ;; ssubst m vs, s) \<Rightarrow>\<^bsup> z \<^esup> t" by simp
-  then obtain z' where *: "Suc (Suc z') = z" and **: "(ssubst m vs, s(m v := s v)) \<Rightarrow>\<^bsup> z' \<^esup> t" by auto
-  from Cons have ***: "\<forall>v\<in>set vs. m v \<notin> set vs" by simp
-  from Cons have ****: "inj_on m (set vs)" by simp
-  from Cons.IH[OF ** **** ***] have step: "s(m v := s v) = t \<circ> m on set vs" and z: "z' = Suc (2 * length vs)" by auto
+  have 1: "(Assign (m v) (A (V v)),s) \<Rightarrow>\<^bsup>Suc (Suc 0) \<^esup> s(m v := s v)"
+    using Assign[of _ "A (V v)"] by simp
+  from Cons obtain t where
+    2: "(ssubst m vs, s(m v := s v)) \<Rightarrow>\<^bsup>Suc (2 * length (vs)) \<^esup> t" and 
+    s: "s(m v := s v) = t \<circ> m on set vs" by fastforce
   hence "s(m v := s v) = t \<circ> m on set (v#vs)"
   proof (cases "v\<in>set vs")
-    case True
-    then show ?thesis
-      using local.step by auto
+    case True then show ?thesis using s by auto
   next
     case False
-    with Cons.prems(3) have a: "v \<notin> set (vars (ssubst m vs))" by (induction vs) auto
+    with Cons.prems(2) have a: "v \<notin> set (vars (ssubst m vs))" by (induction vs) auto
     hence " v \<notin> m ` set vs" by fastforce
     with False have "m v \<notin> m ` set vs" using \<open>\<forall>va\<in>set (v # vs). m va \<notin> set (v # vs)\<close>
-      using Cons.prems(2) by force
+      using Cons.prems(1) by force
     with a have "m v \<notin> set (vars (ssubst m vs))" apply auto 
-      using Cons.prems(3) by force
-    hence "(s(m v := s v)) (m v) = t (m v)" using var_unchanged apply auto
-      using "**" by fastforce
-    then show ?thesis using step by auto
+      using Cons.prems(2) by force
+    hence "(s(m v := s v)) (m v) = t (m v)" using var_unchanged[OF 2] by blast
+    then show ?thesis using s by auto
   qed
-  from z have "z = Suc (2 * length (v # vs))"
-    using "*" by force
-  then show ?case
-    by (metis Cons.prems(3) \<open>s(m v := s v) = t \<circ> m on set (v # vs)\<close> fun_upd_other list.set_intros(1))
+  hence "s = t \<circ> m on set (v # vs)"
+    by (metis Cons.prems(2) fun_upd_other list.set_intros(1))
+  with 1 2 show ?case by fastforce
 qed auto
 
-lemma ssubst_complete:
-  "\<down>(ssubst m vs,s)"
-  by (induction vs arbitrary: s) fastforce+
 
-corollary subst_sound:
-  "\<lbrakk>(c,s) \<Rightarrow>\<^bsup>z\<^esup> t; s = s' o m on set (vars c) ; inj_on m (set (vars c)); (subst m c,s') \<Rightarrow>\<^bsup>z'\<^esup> t'\<rbrakk>
-     \<Longrightarrow> t = t' o m on set (vars c) \<and> z = z'"
-  using big_step_subst by blast
+subsection "Command transfer"
 
 definition [simp]: "transfer m c = ssubst m (vars c);;subst m c"
 
 lemma set_transfer[simp]: "set (vars (transfer m c)) = set (vars c) \<union> m ` set (vars c)"
   unfolding transfer_def by auto
 
-
 lemma transfer_sound:
   assumes c_sem: "(c,s) \<Rightarrow>\<^bsup>z\<^esup> t"
       and s: "s = s' on set (vars c)"
-      and transfer_sem: "(transfer m c,s')\<Rightarrow>\<^bsup>z'\<^esup> t'"
       and inj: "inj_on m (set (vars c))"
       and disj: "(\<forall>v\<in>set (vars c). m v \<notin> set (vars c))"
-    shows "t = t' o m on set (vars c) \<and> Suc (2 * length (vars c)) + z = z'"
-      and "s' = t' on UNIV - m ` set (vars c)"
+    obtains t'
+    where "(transfer m c,s')\<Rightarrow>\<^bsup>Suc (2 * length (vars c)) + z\<^esup> t'"
+      and "t = t' o m on set (vars c)"
 proof -
-  from transfer_sem obtain s'' x y where ssubst_sem: "(ssubst m (vars c),s')\<Rightarrow>\<^bsup>x\<^esup> s''" and subst_sem: "(subst m c,s'') \<Rightarrow>\<^bsup>y\<^esup> t'" "x + y = z'"
-    unfolding transfer_def by blast
-  show "t = t' o m on set (vars c) \<and> Suc (2 * length (vars c)) + z = z'" using ssubst_sound[OF ssubst_sem inj disj] subst_sound[OF c_sem _ inj subst_sem(1)]
-    using s subst_sem(2) by force
-  have "s' = s'' on UNIV - m ` set (vars c)"
-    using disj ssubst_sem ssubst_unchanged
-    by (simp add: rvars_unchanged)
-  moreover have "s'' = t'  on UNIV - m ` set (vars c)" using var_unchanged apply auto
-    using subst_sem(1) by auto
-  ultimately show "s' = t' on UNIV - m ` set (vars c)" by auto
+  from ssubst_correct[OF inj disj] obtain s\<^sub>2 where ssubst_sem:
+    "(ssubst m (vars c),s')\<Rightarrow>\<^bsup>Suc (2 * length (vars c))\<^esup> s\<^sub>2" and
+    "s' = s\<^sub>2 \<circ> m on set (vars c)" by auto
+  with s have s\<^sub>2: "s = s\<^sub>2 o m on set (vars c)" by simp
+
+  from subst_sound[OF c_sem this _ inj] obtain t' where 
+    subst_sem: "(subst m c, s\<^sub>2) \<Rightarrow>\<^bsup> z \<^esup> t'" and t': "t = t' \<circ> m on set (vars c)" by auto
+  with ssubst_sem have "(transfer m c,s')\<Rightarrow>\<^bsup>Suc (2 * length (vars c)) + z\<^esup> t'" by auto
+
+  with t' that show ?thesis by blast  
 qed
 
 lemma transfer_complete:
-  assumes c_sem: "(c,s) \<Rightarrow>\<^bsup>z\<^esup> t"
-      and s: "s = s' on set (vars c)"
+  assumes transfer_sem: "(transfer m c,s')\<Rightarrow>\<^bsup>z'\<^esup> t'"
+      and s: "s' = s on set (vars c)"
       and inj: "inj_on m (set (vars c))"
       and disj: "(\<forall>v\<in>set (vars c). m v \<notin> set (vars c))"
-    shows "\<down>(transfer m c,s')"
+  obtains t z
+    where "(c,s) \<Rightarrow>\<^bsup>z\<^esup> t" "z' = Suc (2 * length (vars c)) + z" "t = t' o m on set (vars c)"
 proof -
-  from ssubst_complete have "\<down>(ssubst m (vars c), s')" by simp
-  then obtain s'' x where ssubst_sem: "(ssubst m (vars c),s')\<Rightarrow>\<^bsup>x\<^esup> s''" by auto
-  from ssubst_sound have "s' = s'' \<circ> m on set (vars c)" using assms ssubst_sem by blast
-  with c_sem have "\<down>(subst m c,s'')" using subst_complete
-    by (metis inj order_refl s)
-  with ssubst_sem show ?thesis
-    unfolding transfer_def by auto
+  from ssubst_correct[OF inj disj] obtain s\<^sub>2' where
+     s\<^sub>2': "(ssubst m (vars c), s') \<Rightarrow>\<^bsup> Suc (2 * length (vars c)) \<^esup> s\<^sub>2'" "s' = s\<^sub>2' \<circ> m on set (vars c)"
+    by auto
+  with transfer_sem[unfolded transfer_def] obtain z where 
+   subst_sem: "(subst m c,s\<^sub>2') \<Rightarrow>\<^bsup>z\<^esup> t'" and z: "z' = Suc (2 * length (vars c)) + z" 
+    using big_step_t_determ2 by fastforce
+  from s s\<^sub>2' have "s = s\<^sub>2' o m on set (vars c)" by simp
+  from subst_complete[OF subst_sem this _ inj] that z show ?thesis by auto
 qed
 
-context notes Let_def[simp] begin
-definition [simp]: "inline1 S c r = (let m = fresh S in (m r) ::= A (V r);;transfer m c;;r ::= A (V (m r)))"
+lemma transfer_unchanged:
+  assumes transfer_sem: "(transfer m c,s) \<Rightarrow>\<^bsup>z\<^esup> t"    
+      and inj: "inj_on m (set (vars c))"
+      and disj: "(\<forall>v\<in>set (vars c). m v \<notin> set (vars c))"
+    shows "s = t on UNIV - m ` set (vars c)"
+proof -
+  from transfer_sem obtain s\<^sub>2 x y where ssubst_sem: "(ssubst m (vars c),s)\<Rightarrow>\<^bsup>x\<^esup> s\<^sub>2" and subst_sem: "(subst m c,s\<^sub>2)\<Rightarrow>\<^bsup>y\<^esup> t" by auto
+  from ssubst_correct[OF inj disj] have "s = s\<^sub>2 o m on set (vars c)"
+    using \<open>(ssubst m (vars c), s) \<Rightarrow>\<^bsup> x \<^esup> s\<^sub>2\<close> bigstep_det by blast
+
+  have "s = s\<^sub>2 on UNIV - m ` set (vars c)"
+    using disj ssubst_sem ssubst_unchanged
+    by (simp add: rvars_unchanged)
+  moreover have "s\<^sub>2 = t  on UNIV - m ` set (vars c)" using var_unchanged apply auto
+    using subst_sem(1) by auto
+  ultimately show "s = t on UNIV - m ` set (vars c)" by auto
+qed
+ 
+definition [simp]: "inline1 S c r =  (fresh S r) ::= A (V r);;transfer (fresh S) c;;r ::= A (V ((fresh S) r))"
 
 lemma inline1_vars_c[simp]: "set (vars c) \<subseteq> set (vars (inline1 S c r))"
   unfolding inline1_def by auto
@@ -212,108 +226,136 @@ lemma inline1_vars_c[simp]: "set (vars c) \<subseteq> set (vars (inline1 S c r))
 lemma inline1_vars_r[simp]: "r \<in> set (vars (inline1 S c r))"
   unfolding inline1_def by auto
 
+lemma inline1_unchanged:
+  assumes inline1_sem: "(inline1 S c r,s) \<Rightarrow>\<^bsup>z\<^esup> t"
+      and S: "set (r#vars c) \<subseteq> set S"
+    shows "s = t on set S - {r}"
+proof -
+  let ?m = "fresh S"
+  have inj: "inj_on ?m (set (vars c))" and disj: "(\<forall>v\<in>set (vars c). ?m v \<notin> set (vars c))"
+    using S fresh fresh_inj inj_on_subset by auto
+  
+  from inline1_sem obtain s\<^sub>1 z\<^sub>1 z\<^sub>2  s\<^sub>2 z z\<^sub>3 where
+    to_sem: "((?m r) ::= A (V r),s) \<Rightarrow>\<^bsup>z\<^sub>1\<^esup> s\<^sub>1" and
+    "(transfer ?m c;;r ::= A (V (?m r)),s\<^sub>1)\<Rightarrow>\<^bsup>z\<^sub>2\<^esup> t" and
+    transfer_sem: "(transfer ?m c,s\<^sub>1)\<Rightarrow>\<^bsup>z\<^esup> s\<^sub>2" and
+    from_sem: "(r ::= A (V (?m r)),s\<^sub>2)\<Rightarrow>\<^bsup>z\<^sub>3\<^esup> t"
+    unfolding inline1_def by fastforce
+  
+  hence s\<^sub>1: "s\<^sub>1 = s(?m r := s r)" "t = s\<^sub>2(r := s\<^sub>2(?m r))" by auto
+  moreover have "s\<^sub>1 = s\<^sub>2 on set S" using transfer_unchanged[OF transfer_sem inj disj] by auto
+
+  ultimately show "s = t on set S - {r}"
+    by (metis DiffE fresh fun_upd_other singleton_iff)
+qed
+
 lemma inline1_sound:
   assumes c_sem: "(c,s) \<Rightarrow>\<^bsup>z\<^esup> t"
       and s: "s = s' on set (r#vars c)"
       and S: "set (r#vars c) \<subseteq> set S"
-      and inline1_sem: "(inline1 S c r,s') \<Rightarrow>\<^bsup>zr\<^esup> tr"
-    shows "t r = tr r" and "s' = tr on set S - {r}" and "2 * length (vars c) + z + 5 = zr"
+  obtains zr tr
+    where "(inline1 S c r,s') \<Rightarrow>\<^bsup>zr\<^esup> tr"  
+      and "t r = tr r" "2 * length (vars c) + z + 5 = zr"
 proof -
-  let ?m = "fresh S"
-  have inj: "inj_on ?m (set (vars c))"
-    using S fresh_inj inj_on_subset by auto
-  have disj: "(\<forall>v\<in>set (vars c). ?m v \<notin> set (vars c))"
-    using S fresh by auto
+  let ?m = "fresh S" let ?s\<^sub>1' = "s'((?m r) := s' r)" let ?z' = "Suc (2 * length (vars c)) + z"
+
+  have inj: "inj_on ?m (set (vars c))" using S fresh_inj inj_on_subset by auto
+  have disj: "(\<forall>v\<in>set (vars c). ?m v \<notin> set (vars c))" using S fresh by auto
   
-  from inline1_sem obtain s\<^sub>1' z\<^sub>1' z\<^sub>2' where def1: 
-    "((?m r) ::= A (V r),s') \<Rightarrow>\<^bsup>z\<^sub>1'\<^esup> s\<^sub>1'"
-    "(transfer ?m c;;r ::= A (V (?m r)),s\<^sub>1')\<Rightarrow>\<^bsup>z\<^sub>2'\<^esup> tr"
-    "z\<^sub>1' + z\<^sub>2' = zr"
-    unfolding inline1_def by fastforce
-  from def1(2) obtain s\<^sub>2' z' z\<^sub>3' where def2:
-    "(transfer ?m c,s\<^sub>1')\<Rightarrow>\<^bsup>z'\<^esup> s\<^sub>2'"
-    "(r ::= A (V (?m r)),s\<^sub>2')\<Rightarrow>\<^bsup>z\<^sub>3'\<^esup> tr"
-    "z' + z\<^sub>3' = z\<^sub>2'"
-    by fastforce    
+  have 1: "((?m r) ::= A (V r),s') \<Rightarrow>\<^bsup>Suc (Suc 0)\<^esup> ?s\<^sub>1'"
+    using big_step_t.Assign[of "?m r" "A (V r)" s'] by auto
+  have s\<^sub>1': "s = ?s\<^sub>1' on set (vars c)" using S s by auto
 
-  from def1(1) have "z\<^sub>1' = Suc (Suc 0)" and s\<^sub>1': "s\<^sub>1' = s'(?m r := s' r)" by auto
-  from s have s': "s=s\<^sub>1' on set (vars c)"
-    using S s\<^sub>1' by auto
-  from def2(1) have **:"t = s\<^sub>2' o ?m on set (vars c) \<and> Suc (2 * length (vars c)) + z = z'" 
-    and ***: "s\<^sub>1' = s\<^sub>2' on UNIV - ?m ` set (vars c)"
-    using transfer_sound[OF c_sem s' _ inj disj] by auto
-
-  from def2 have "z\<^sub>3' = Suc (Suc 0)" and tr: "tr = s\<^sub>2'(r := s\<^sub>2'(?m r))" by auto
-
-  have "zr = Suc (Suc 0) + Suc (2 * length (vars c)) + z + Suc (Suc 0)"
-    using \<open>z\<^sub>1' = Suc (Suc 0)\<close> \<open>z\<^sub>3' = Suc (Suc 0)\<close> def1(3) def2(3) ** by auto
-  from this[symmetric] show "2 * length (vars c) + z + 5 = zr" by linarith
-
-  from def2 have "tr r = (s\<^sub>2' o ?m) r" by auto
-  show "t r = tr r"
+  obtain s\<^sub>2' where 
+    2: "(transfer ?m c, ?s\<^sub>1') \<Rightarrow>\<^bsup>?z'\<^esup> s\<^sub>2'" and s\<^sub>2': "t = s\<^sub>2' \<circ> ?m on set (vars c)"
+    using transfer_sound[OF c_sem s\<^sub>1' inj disj] by blast
+  
+  then obtain tr where 
+    3: "(r ::= A (V (?m r)),s\<^sub>2')\<Rightarrow>\<^bsup>Suc (Suc 0)\<^esup> tr" and tr: "tr = s\<^sub>2'(r := s\<^sub>2'(?m r))"
+    by fastforce
+  
+  from 1 2 3 s\<^sub>1' have res: "(inline1 S c r,s')\<Rightarrow>\<^bsup>Suc (Suc 0) + ?z' + Suc (Suc 0)\<^esup> tr"
+    unfolding inline1_def using Seq by meson
+ 
+  have "t r = tr r"
   proof (cases "r \<in> set (vars c)")
     case True
-    then show ?thesis
-      by (simp add: "**" \<open>tr r = (s\<^sub>2' \<circ> fresh S) r\<close>)
+    from tr have "tr r = (s\<^sub>2' o ?m) r" by auto
+    with True show ?thesis using s\<^sub>2' by simp
   next
     case False
     hence "?m r \<notin> set (vars (transfer ?m c))"
       by (smt (verit, best) S Un_iff fresh fresh_inj inj_on_image_mem_iff list.set_intros(1) set_subset_Cons set_transfer subsetD subset_inj_on)
     
-    with def2(1) have "s\<^sub>1' (?m r) = s\<^sub>2' (?m r)"
+    with 2 have "?s\<^sub>1' (?m r) = s\<^sub>2' (?m r)"
       using var_unchanged by blast
 
-    then show ?thesis
-      by (metis False c_sem fun_upd_same list.set_intros(1) s s\<^sub>1' tr var_unchanged)
+    then show ?thesis by (metis False c_sem fun_upd_same list.set_intros(1) s tr var_unchanged)
   qed
-
-  from *** have "s\<^sub>1' = s\<^sub>2' on set S" by auto
-
-  show "s' = tr on set S - {r}"
-    by (metis DiffE \<open>s\<^sub>1' = s\<^sub>2' on set S\<close> fresh fun_upd_other s\<^sub>1' singleton_iff tr)
+  then show ?thesis using that res by auto
 qed
 
 lemma inline1_complete:
-    assumes c_sem: "(c,s) \<Rightarrow>\<^bsup>z\<^esup> t"
+  assumes inline_sem: "(inline1 S c r,s') \<Rightarrow>\<^bsup>zr\<^esup> tr" 
       and s: "s = s' on set (r#vars c)"
-      and S: "set (r#vars c) \<subseteq> set S"
-    shows "\<down>(inline1 S c r,s')"
+      and S: "set (r#vars c) \<subseteq> set S" 
+  obtains z t
+    where "(c,s) \<Rightarrow>\<^bsup>z\<^esup> t \<and> tr r = t r \<and> 2 * length (vars c) + z + 5 = zr"
 proof -
-  let ?m = "fresh S"
-  have inj: "inj_on ?m (set (vars c))"
-    using S fresh_inj inj_on_subset by auto
-  have disj: "(\<forall>v\<in>set (vars c). ?m v \<notin> set (vars c))"
-    using S fresh by auto
+  let ?m = "fresh S" let ?s\<^sub>1' = "s'((?m r) := s' r)"
 
-  have 1: "((?m r) ::= A (V r),s') \<Rightarrow>\<^bsup>Suc (Suc 0)\<^esup> s'((?m r) := s' r)"
-    using big_step_t.Assign[of "?m r" "A (V r)" s'] by auto
-
-  have s': "s = s'((?m r) := s' r) on set (vars c)"
-    using S s by auto
-
-  have 2: "\<down> (transfer (fresh S) c, s'(fresh S r := s' r))"
-    using transfer_complete[OF c_sem s' inj disj] .
-
-  hence 3: "\<down> (transfer (fresh S) c;;r ::= A (V (?m r)), s'(fresh S r := s' r))" by auto
-  then obtain z t where "(transfer (fresh S) c;;r ::= A (V (?m r)), s'(fresh S r := s' r))\<Rightarrow>\<^bsup>z\<^esup> t" by blast
+  have inj: "inj_on ?m (set (vars c))" using S fresh_inj inj_on_subset by auto
+  have disj: "(\<forall>v\<in>set (vars c). ?m v \<notin> set (vars c))" using S fresh by auto
   
-  with 1 s' have "((?m r) ::= A (V r);;transfer ?m c;;r ::= A (V (?m r)),s')\<Rightarrow>\<^bsup>Suc (Suc 0) + z\<^esup> t"
-    by (smt (verit, best) Seq_tE add.assoc compose_programs_2)
+  have 1: "((?m r) ::= A (V r),s') \<Rightarrow>\<^bsup>Suc (Suc 0)\<^esup> ?s\<^sub>1'"
+    using big_step_t.Assign[of "?m r" "A (V r)" s'] by auto
+  have s\<^sub>1': "?s\<^sub>1' = s on set (vars c)" using S s by auto
 
-  then show ?thesis unfolding inline1_def by fastforce
+  from inline_sem obtain t' z' where 
+    2: "(transfer ?m c,?s\<^sub>1') \<Rightarrow>\<^bsup>z'\<^esup> t'" and z': "z' + 4 = zr" by fastforce
+  from transfer_complete[OF 2 s\<^sub>1' inj disj] obtain t z where 
+    c_sem: "(c, s) \<Rightarrow>\<^bsup> z \<^esup> t" and 
+    z: "z' = Suc (2 * length (vars c)) + z" and 
+    t: "t = t' \<circ> fresh S on set (vars c)" by metis
+
+  obtain tr' where
+    3: "(r ::= A (V (?m r)),t')\<Rightarrow>\<^bsup>Suc (Suc 0)\<^esup> tr'" and tr: "tr' = t'(r := t'(?m r))" 
+    by fastforce
+
+  moreover from z have "(inline1 S c r,s')\<Rightarrow>\<^bsup>Suc (Suc 0) + Suc (2 * length (vars c)) + z + Suc (Suc 0)\<^esup> tr'" 
+    unfolding inline1_def using Seq[OF 1 2] Seq[OF _ 3] by auto
+
+  ultimately have tr': "tr' = tr"
+    using bigstep_det inline_sem by blast
+
+  have "tr' r = t r"
+  proof (cases "r \<in> set (vars c)")
+    case True
+    from tr have "tr' r = (t' o ?m) r" by auto
+    with True show ?thesis using t by simp
+  next
+    case False
+    hence "?m r \<notin> set (vars (transfer ?m c))"
+      by (smt (verit, best) S Un_iff fresh fresh_inj inj_on_image_mem_iff list.set_intros(1) set_subset_Cons set_transfer subsetD subset_inj_on)
+    
+    with 2 have "?s\<^sub>1' (?m r) = t' (?m r)"
+      using var_unchanged by blast
+
+     show ?thesis
+       by (metis False \<open>(s'(fresh S r := s' r)) (fresh S r) = t' (fresh S r)\<close> c_sem fun_upd_same list.set_intros(1) s tr var_unchanged)
+   qed
+
+  then show ?thesis using that c_sem z z' tr' by auto
 qed
+
+
+section \<open>Program inlining\<close>
 
 fun inline_S :: "vname list \<Rightarrow> com' \<Rightarrow> com" where
   "inline_S S SKIP' = SKIP" |
   "inline_S S (Assign' x a) = (x::=a)" |
-  "inline_S S (Seq' c\<^sub>1' c\<^sub>2') = (let
-    c\<^sub>1 = inline_S S c\<^sub>1';
-    c\<^sub>2 = inline_S (S @ vars c\<^sub>1) c\<^sub>2'
-  in c\<^sub>1;;c\<^sub>2)" |
-  "inline_S S (If' b c\<^sub>1' c\<^sub>2') = (let
-    c\<^sub>1 = inline_S S c\<^sub>1';
-    c\<^sub>2 = inline_S S c\<^sub>2'
-  in IF b\<noteq>0 THEN c\<^sub>1 ELSE c\<^sub>2)" |
+  "inline_S S (Seq' c\<^sub>1' c\<^sub>2') = inline_S S c\<^sub>1';;inline_S S c\<^sub>2'" |
+  "inline_S S (If' b c\<^sub>1' c\<^sub>2') = IF b\<noteq>0 THEN inline_S S c\<^sub>1' ELSE inline_S S c\<^sub>2'" |
   "inline_S S (While' b c') = WHILE b\<noteq>0 DO inline_S S c'" |  
   "inline_S S (Call' c r) = inline1 S c r"
 
@@ -321,137 +363,139 @@ lemma vars_inline_S[simp]: "set (vars c) \<subseteq> set (vars (inline_S S c))"
   by (induction c arbitrary: S) auto
 
 lemma inline_S_sound: 
-  "\<lbrakk> (c',s') \<Rightarrow>'\<^bsup>z'\<^esup> t'; s'= s on T; set (vars c') \<subseteq> set S; set (vars c') \<subseteq> T; T \<subseteq> set S; (inline_S S c',s)\<Rightarrow>\<^bsup>z\<^esup> t \<rbrakk>
-    \<Longrightarrow> t = t' on T \<and> z \<le> z' + (z' + 1) * size\<^sub>c c'"
-proof(induction c' s' z' t' arbitrary: S s z t rule: big_step_t'_induct)
-  case (Assign x a s)
-  then show ?case by (auto simp: subset_iff)
+  "\<lbrakk> (c',s') \<Rightarrow>'\<^bsup>z'\<^esup> t'; s'= s on set S; set (vars c') \<subseteq> set S \<rbrakk>
+    \<Longrightarrow> \<exists>t z. (inline_S S c',s)\<Rightarrow>\<^bsup>z\<^esup> t \<and> t = t' on set S \<and> z \<le> z' + (z' + 1) * size\<^sub>c c'"
+proof(induction c' s' z' t' arbitrary: s rule: big_step_t'_induct)
+  case (Assign' x a s' s)
+  hence "s(x := aval a s) = s'(x := aval a s') on set S" by (auto simp: in_mono)
+  moreover have "(inline_S S (Assign' x a), s) \<Rightarrow>\<^bsup> Suc (Suc 0) \<^esup> s(x := aval a s)" by auto
+  ultimately show ?case by fastforce
 next
-  case (Seq c\<^sub>1' s\<^sub>1' x' s\<^sub>2' c\<^sub>2' y' s\<^sub>3' z' S s\<^sub>1 z t)
-  let ?S = "(S @ vars (inline_S S c\<^sub>1'))"
-  from Seq obtain s\<^sub>2 x s\<^sub>3 y where "(inline_S S c\<^sub>1' ,s\<^sub>1) \<Rightarrow>\<^bsup>x\<^esup> s\<^sub>2" and 2:"(inline_S ?S c\<^sub>2' ,s\<^sub>2) \<Rightarrow>\<^bsup>y\<^esup> s\<^sub>3" and "x + y = z" by auto
-  with Seq have s2: "s\<^sub>2' = s\<^sub>2 on T" and t2: "x \<le> x' + (x' + 1) * size\<^sub>c c\<^sub>1'" apply auto by fastforce
-  have "set (vars c\<^sub>2') \<subseteq> set (S @ vars (inline_S S c\<^sub>1'))"
-    using Seq.prems(2) by force
-  with Seq.IH(2)[OF s2 _ _ _ 2]  have "s\<^sub>3 = s\<^sub>3' on T" and t3: " y \<le> y' + (y' + 1) * size\<^sub>c c\<^sub>2'" apply auto
-    using Seq.prems(3) \<open>set (vars c\<^sub>2') \<subseteq> set (S @ vars (inline_S S c\<^sub>1'))\<close>  apply auto
-    using Seq.prems(4) apply blast+ done
-  have *: " t = s\<^sub>3' on T"
-    by (smt (verit, ccfv_SIG) "2" Seq.prems(5) \<open>(inline_S S c\<^sub>1', s\<^sub>1) \<Rightarrow>\<^bsup> x \<^esup> s\<^sub>2\<close> \<open>s\<^sub>3 = s\<^sub>3' on T\<close> big_step_t.Seq big_step_t_determ2 inline_S.simps(3))
-
-  from Seq.hyps have "x' + y' = z'" by simp
-  with \<open>x + y = z\<close> t2 t3
-  have **: "z \<le> z' + (z' + 1) * (size\<^sub>c c\<^sub>1' + size\<^sub>c c\<^sub>2')" by (auto simp: algebra_simps)
-
-  from * ** show ?case by simp
+  case (Seq' c\<^sub>1 s\<^sub>1 x s\<^sub>2 c\<^sub>2 y s\<^sub>3 z s\<^sub>1')
+  then obtain s\<^sub>2' x' where 
+    1: "(inline_S S c\<^sub>1, s\<^sub>1') \<Rightarrow>\<^bsup> x' \<^esup> s\<^sub>2' \<and> s\<^sub>2' = s\<^sub>2 on set S \<and> x' \<le> x + (x + 1) * size\<^sub>c c\<^sub>1"
+    by fastforce
+  hence prems2: "s\<^sub>2 = s\<^sub>2' on set S" by auto
+  from Seq' obtain s\<^sub>3' y' where 
+    2: "(inline_S S c\<^sub>2, s\<^sub>2') \<Rightarrow>\<^bsup> y' \<^esup> s\<^sub>3' \<and> s\<^sub>3' = s\<^sub>3 on set S \<and> y' \<le> y + (y + 1) * size\<^sub>c c\<^sub>2"
+    using Seq'.IH(2)[OF prems2 ] by auto
+  from 1 2 Seq'.hyps(3) show ?case by (fastforce simp: algebra_simps)
 next
-  case (IfTrue s' b c\<^sub>1' x' t' y' c\<^sub>2' S s y t) 
-  then obtain x where step: "(inline_S S c\<^sub>1' ,s) \<Rightarrow>\<^bsup>x\<^esup> t" and y_def: "1 + x = y" by auto
-  from IfTrue have prems: "set (vars c\<^sub>1') \<subseteq> set S" "set (vars c\<^sub>1') \<subseteq> T" by auto
-  from IfTrue.IH[OF IfTrue.prems(1) prems IfTrue.prems(4) step] have "t = t' on T \<and> x \<le> x' + (x' + 1) * size\<^sub>c c\<^sub>1'" .
-  with y_def IfTrue.hyps(3) show ?case by (auto simp: algebra_simps)
+  case (IfTrue' s b c\<^sub>1' x t y c\<^sub>2' s')
+  then obtain x' t' where "(inline_S S c\<^sub>1', s') \<Rightarrow>\<^bsup> x' \<^esup> t' \<and> t' = t on set S \<and> x' \<le> x + (x + 1) * size\<^sub>c c\<^sub>1'" by fastforce
+  with IfTrue'.hyps(1,3) IfTrue'.prems have 
+    "(inline_S S (If' b c\<^sub>1' c\<^sub>2'), s') \<Rightarrow>\<^bsup> x' + 1 \<^esup> t' \<and> t' = t on set S \<and> x' + 1 \<le> y + (y + 1) * size\<^sub>c (If' b c\<^sub>1' c\<^sub>2')"
+    by (auto simp: algebra_simps)
+  thus ?case by blast
 next
-  case (IfFalse s' b c\<^sub>2' x' t' y' c\<^sub>1' S s y t) 
-  then obtain x where step: "(inline_S S c\<^sub>2' ,s) \<Rightarrow>\<^bsup>x\<^esup> t" and y_def: "1 + x = y" by auto
-  from IfFalse have prems: "set (vars c\<^sub>2') \<subseteq> set S" "set (vars c\<^sub>2') \<subseteq> T" by auto
-  from IfFalse.IH[OF IfFalse.prems(1) prems IfFalse.prems(4) step] have "t = t' on T \<and> x \<le> x' + (x' + 1) * size\<^sub>c c\<^sub>2'" .
-  with y_def IfFalse.hyps(3) show ?case by (auto simp: algebra_simps)
+  case (IfFalse' s b c\<^sub>2' x t y c\<^sub>1' s')
+  then obtain x' t' where "(inline_S S c\<^sub>2', s') \<Rightarrow>\<^bsup> x' \<^esup> t' \<and> t' = t on set S \<and> x' \<le> x + (x + 1) * size\<^sub>c c\<^sub>2'" by fastforce
+  with IfFalse'.hyps(1,3) IfFalse'.prems have 
+    "(inline_S S (If' b c\<^sub>1' c\<^sub>2'), s') \<Rightarrow>\<^bsup> x' + 1 \<^esup> t' \<and> t' = t on set S \<and> x' + 1 \<le> y + (y + 1) * size\<^sub>c (If' b c\<^sub>1' c\<^sub>2')"
+    by (auto simp: algebra_simps)
+  thus ?case by blast
 next
-  case (WhileTrue s\<^sub>1' b c' x' s\<^sub>2' y' s\<^sub>3' z' S s\<^sub>1 z s\<^sub>3) thm WhileTrue.prems
-  then obtain x y s\<^sub>2 where step: 
-    "(inline_S S c',s\<^sub>1)\<Rightarrow>\<^bsup>x\<^esup> s\<^sub>2" 
-    "(inline_S S (While' b c'), s\<^sub>2) \<Rightarrow>\<^bsup> y \<^esup> s\<^sub>3"
-  and z_def: "1 + x + y = z" by auto
-  from WhileTrue have prems: 
-    "set (vars c') \<subseteq> set S" "set (vars c') \<subseteq> T"
-    "set (vars (While' b c')) \<subseteq> set S" "set (vars (While' b c')) \<subseteq> T" by auto
-  from WhileTrue.IH(1)[OF WhileTrue.prems(1) prems(1,2) WhileTrue.prems(4) step(1)]
-  have "s\<^sub>2' = s\<^sub>2 on T" "x \<le> x' + (x' + 1) * size\<^sub>c c'" by auto
-  moreover from WhileTrue.IH(2)[OF this(1) prems(3,4) WhileTrue.prems(4) step(2)]
-  have "s\<^sub>3 = s\<^sub>3' on T" " y \<le> y' + (y' + 1) * size\<^sub>c (While' b c')" by auto
-  ultimately show ?case using z_def WhileTrue.hyps(4) by (auto simp: algebra_simps)
+  case (WhileTrue' s\<^sub>1 b c\<^sub>1 x s\<^sub>2 y s\<^sub>3 z s\<^sub>1')
+  hence prems1: "set (vars c\<^sub>1) \<subseteq> set S" by simp
+  obtain s\<^sub>2' x' where 1: "(inline_S S c\<^sub>1, s\<^sub>1') \<Rightarrow>\<^bsup> x' \<^esup> s\<^sub>2' \<and> s\<^sub>2' = s\<^sub>2 on set S \<and> x' \<le> x + (x + 1) * size\<^sub>c c\<^sub>1"
+    using WhileTrue'.IH(1)[OF WhileTrue'.prems(1) prems1] by blast
+  with WhileTrue' have prems2: "s\<^sub>2 = s\<^sub>2' on set S" "set (vars (While' b c\<^sub>1)) \<subseteq> set S" by auto
+  obtain s\<^sub>3' y' where 2: "(inline_S S (While' b c\<^sub>1), s\<^sub>2') \<Rightarrow>\<^bsup> y' \<^esup> s\<^sub>3' \<and> s\<^sub>3' = s\<^sub>3 on set S \<and> y' \<le> y + (y + 1) * size\<^sub>c (While' b c\<^sub>1)"
+    using WhileTrue'.IH(2)[OF prems2] by auto
+  from WhileTrue' have "s\<^sub>1' b \<noteq> 0" by simp 
+  with 1 2 WhileTrue'.hyps(4) have "(inline_S S (While' b c\<^sub>1), s\<^sub>1') \<Rightarrow>\<^bsup> 1 + x' + y' \<^esup> s\<^sub>3' \<and> s\<^sub>3' = s\<^sub>3 on set S \<and> 1 + x' + y' \<le> z + (z + 1) * size\<^sub>c (While' b c\<^sub>1)"
+    by (auto simp: algebra_simps)
+  thus ?case by blast
 next
-  case (Call c s z t s' r S s'' z' t')
-
-  from Call have prems: "s = s'' on set (r # vars c)" "set (r # vars c) \<subseteq> set S" "(inline1 S c r, s'') \<Rightarrow>\<^bsup> z' \<^esup> t'" by auto
-
-  have tr: "t r = t' r" and t: "2 * length (vars c) + z + 5 = z'" using inline1_sound[OF \<open>(c, s) \<Rightarrow>\<^bsup> z \<^esup> t\<close> prems] by auto
-
-  from Call.hyps(1) prems(3) have "t' = s''(r := t' r) on T"
-    by (smt (verit, ccfv_SIG) Call.prems(4) DiffI empty_iff fun_upd_apply inline1_sound(2) insert_iff prems(1) prems(2) subsetD)
-
-  with tr Call have "t' = s'(r := t r) on T" by fastforce
-  with t show ?case by simp
+  case (Call' c s z t r s')
+  hence prems: "s = s' on set (r # vars c)" "set (r # vars c) \<subseteq> set S" by auto
+  then obtain zr tr where 
+    inline: "(inline1 S c r, s') \<Rightarrow>\<^bsup> zr \<^esup> tr" "t r = tr r" "2 * length (vars c) + z + 5 = zr" 
+    using inline1_sound[OF Call'.hyps] by blast
+  with Call'.prems(1) inline1_unchanged[OF inline(1) prems(2)] have "tr = s(r := tr r) on set S"
+    by simp
+  with inline have " (inline_S S (Call' c r), s') \<Rightarrow>\<^bsup> zr \<^esup> tr \<and> tr = s(r := t r) on set S \<and> zr \<le> z + (z + 1) * size\<^sub>c (Call' c r)" by simp
+  then show ?case by blast
 qed auto
 
 lemma inline_S_complete:
-  "\<lbrakk> (c',s') \<Rightarrow>'\<^bsup>z'\<^esup> t'; s'= s on T; set (vars c') \<subseteq> set S; set (vars c') \<subseteq> T; T \<subseteq> set S \<rbrakk>
-    \<Longrightarrow>  \<down> (inline_S S c',s)"
-proof(induction c' s' z' t' arbitrary: S s rule: big_step_t'_induct)
-  case (Seq c\<^sub>1' s\<^sub>1' x' s\<^sub>2' c\<^sub>2' y' s\<^sub>3' z' S s\<^sub>1)
-  hence "\<down> (inline_S S c\<^sub>1', s\<^sub>1)" by auto
-  then obtain x s\<^sub>2 where 1: "(inline_S S c\<^sub>1', s\<^sub>1) \<Rightarrow>\<^bsup>x\<^esup> s\<^sub>2" by auto
-  let ?S = "(S @ vars (inline_S S c\<^sub>1'))"
-  from Seq have "s\<^sub>2' = s\<^sub>2 on T" "set (vars c\<^sub>2') \<subseteq> set ?S" "set (vars c\<^sub>2') \<subseteq> T" "T \<subseteq> set ?S"
-    using inline_S_sound[OF \<open> (c\<^sub>1', s\<^sub>1') \<Rightarrow>'\<^bsup> x' \<^esup> s\<^sub>2'\<close> _ _ _ _ 1] by auto
-  with Seq.IH(2) have "\<down> (inline_S ?S c\<^sub>2', s\<^sub>2)" by auto
-  with 1 show ?case by auto 
+  assumes "(inline_S S c',s) \<Rightarrow>\<^bsup>z\<^esup> t" "s= s' on set S" "set (vars c') \<subseteq> set S"
+  shows "\<exists>z' t'. (c',s') \<Rightarrow>'\<^bsup>z'\<^esup> t' \<and> t = t' on set S \<and> z' \<le> z"
+  using assms proof (induction "inline_S S c'" s z t arbitrary: c' s' rule: big_step_t_induct)
+  case (Skip s)
+  then show ?case by (cases c') auto
 next
-  case (IfTrue s b c1 x t y c2)
-  then show ?case apply auto
-    by (metis IfTrue.hyps(1) big_step_t.IfTrue)
+  case (Assign x a s)
+  then show ?case apply (cases c') apply auto
+    by (metis Assign' aval_eq_if_eq_on_vars eq_imp_le fun_upd_apply subset_iff)
 next
-  case (IfFalse s b c2 x t y c1)
-  then show ?case apply auto
-    by (metis big_step_t.IfFalse)
+  case (Seq c\<^sub>1 s\<^sub>1 x s\<^sub>2 c\<^sub>2 y s\<^sub>3 z c')
+  then show ?case
+  proof (cases c')
+    case (Seq' c\<^sub>1' c\<^sub>2') with Seq show ?thesis by fastforce
+  next
+    case (Call' c r)
+    with Seq.prems Seq.hyps(1,3,5,6) have 1: "(inline1 S c r,s\<^sub>1)\<Rightarrow>\<^bsup> z \<^esup> s\<^sub>3"  "s' = s\<^sub>1 on set (r # vars c)" "set (r # vars c) \<subseteq> set S"
+      by auto
+    from inline1_complete[OF this] obtain z' t where 
+      c_sem: "(c, s') \<Rightarrow>\<^bsup> z' \<^esup> t" and t: "s\<^sub>3 r = t r" and z': "2 * length (vars c) + z' + 5 = z" by metis
+    with big_step_t'.Call' Call' have "(c',s') \<Rightarrow>'\<^bsup> z' \<^esup> s'(r := t r)" by simp
+    have "s\<^sub>1 = s\<^sub>3 on set S - {r}" using inline1_unchanged[OF 1(1) 1(3)] .
+    show ?thesis
+      using Seq.prems(1) \<open>(c', s') \<Rightarrow>'\<^bsup> z' \<^esup> s'(r := t r)\<close> \<open>s\<^sub>1 = s\<^sub>3 on set S - {r}\<close> t z' by fastforce
+  qed (use Seq.hyps(6) in auto)
 next
-  case (WhileTrue s\<^sub>1' b c' x' s\<^sub>2' y' s\<^sub>3' z' S s\<^sub>1)
-  hence "\<down> (inline_S S c',s\<^sub>1)" by auto
-  then obtain x s\<^sub>2  where 1: "(inline_S S c', s\<^sub>1) \<Rightarrow>\<^bsup>x\<^esup> s\<^sub>2" by auto
-  from WhileTrue have "s\<^sub>2' = s\<^sub>2 on T" "set (vars (While' b c')) \<subseteq> set S" "set (vars (While' b c')) \<subseteq> T" "T \<subseteq> set S"
-    using inline_S_sound[OF \<open>(c', s\<^sub>1') \<Rightarrow>'\<^bsup> x' \<^esup> s\<^sub>2'\<close> _ _ _ _ 1] by auto
-  with WhileTrue.IH(2) have "\<down> (inline_S S (While' b c'), s\<^sub>2)" by auto
-  with 1 show ?case by auto blast
+  case (IfTrue s b c\<^sub>1 x t y c\<^sub>2)
+  then obtain c\<^sub>1' c\<^sub>2' where c': "c' = If' b c\<^sub>1' c\<^sub>2'" by (cases c') auto
+  with IfTrue obtain x' t' where "(c\<^sub>1', s') \<Rightarrow>'\<^bsup>x'\<^esup> t' \<and> (t = t' on set S) \<and> x' \<le> x" by fastforce
+  with c' IfTrue show ?case by fastforce
 next
-  case (Call c s z t t' r S s')
-  then have prems: "set (r#vars c) \<subseteq> set S" "s = s' on set (r # vars c)" by auto
-  (* why does the unifier not find the s' with just prems? *)
-  show ?case using inline1_complete[OF Call.hyps(1) _ prems(1), of s', OF prems(2)] by simp
-qed auto
-
-end
+  case (IfFalse s b c\<^sub>2 x t y c\<^sub>1)
+  then obtain c\<^sub>1' c\<^sub>2' where c': "c' = If' b c\<^sub>1' c\<^sub>2'" by (cases c') auto
+  with IfFalse obtain x' t' where "(c\<^sub>2', s') \<Rightarrow>'\<^bsup>x'\<^esup> t' \<and> (t = t' on set S) \<and> x' \<le> x" by fastforce
+  with c' IfFalse show ?case by fastforce
+next
+  case (WhileFalse s b c)
+  then show ?case by (cases c') auto
+next
+  case (WhileTrue s\<^sub>1 b c\<^sub>1 x s\<^sub>2 y s\<^sub>3 z c' s\<^sub>1')
+  then obtain c\<^sub>1' where c'[simp]: "c' = While' b c\<^sub>1'" by (cases c') auto
+  with WhileTrue obtain s\<^sub>2' x' where 1: "(c\<^sub>1', s\<^sub>1') \<Rightarrow>'\<^bsup> x' \<^esup> s\<^sub>2' \<and> s\<^sub>2 = s\<^sub>2' on set S \<and> x' \<le> x" by fastforce
+  with WhileTrue c' obtain s\<^sub>3' y' where 2: "(While' b c\<^sub>1', s\<^sub>2') \<Rightarrow>'\<^bsup> y' \<^esup> s\<^sub>3' \<and> s\<^sub>3 = s\<^sub>3' on set S \<and> y' \<le> y" by fastforce
+  from c' WhileTrue.prems WhileTrue.hyps(1) have b: "s\<^sub>1' b \<noteq> 0" by auto
+  with 1 2 c' have "(While' b c\<^sub>1', s\<^sub>1') \<Rightarrow>'\<^bsup> 1 + x' + y' \<^esup> s\<^sub>3'" "1 + x' + y' \<le> 1 + x + y" using WhileTrue'[of s\<^sub>1', OF b] by auto
+  with c' WhileTrue.hyps(6) show ?case using 2 by blast
+qed
 
 definition inline :: "com' \<Rightarrow> com" where
   [simp]: "inline c = inline_S (vars c) c"
 
-corollary inline_sound:
+
+theorem inline_sound:
   assumes c_sem: "(c,s') \<Rightarrow>'\<^bsup>z'\<^esup> t'"
       and s: "s' = s on set (vars c)"
-      and inline_sem: "(inline c,s)\<Rightarrow>\<^bsup>z\<^esup> t"
-    shows "t = t' on set (vars c) \<and> z \<le> z' + (z' + 1) * size\<^sub>c c"
-proof -
-  have S: "set (vars c) \<subseteq> set (vars c)" by auto
-  show ?thesis unfolding inline_def 
-    by (rule inline_S_sound[OF c_sem s S S S inline_sem[unfolded inline_def]])
-qed
-
-corollary inline_complete:
-  assumes c_sem: "(c,s') \<Rightarrow>'\<^bsup>z'\<^esup> t'"
-      and s: "s' = s on set (vars c)"
-    shows "\<down> (inline c,s)"
-proof -
-  have S: "set (vars c) \<subseteq> set (vars c)" by auto
-  show ?thesis unfolding inline_def by (rule inline_S_complete[OF c_sem s S S S])
-qed
-
-text \<open>Final correctness theorem\<close>
-theorem inline_correct:
-  assumes "(c,s') \<Rightarrow>'\<^bsup>z'\<^esup> t'"
-      and "s' = s on set (vars c)"
   obtains z t 
     where "(inline c,s)\<Rightarrow>\<^bsup>z\<^esup> t" 
       and "t = t' on set (vars c)" 
       and "z \<le> (z' + 1) * (1 + size\<^sub>c c)"
-  using assms inline_complete[OF assms] inline_sound[OF assms] by (fastforce simp: algebra_simps)
+  unfolding inline_def using inline_S_sound[OF c_sem s] by auto
+
+theorem inline_complete:
+  assumes inline_sem: "(inline c,s)\<Rightarrow>\<^bsup>z\<^esup> t"
+      and s: "s = s' on set (vars c)"
+  obtains z' t'
+   where "(c,s') \<Rightarrow>'\<^bsup>z'\<^esup> t'"
+     and "t = t' on set (vars c)" "z' \<le> z"
+  unfolding inline_def using inline_S_complete[OF inline_sem[unfolded inline_def] s] by auto
+
+
+text \<open>Final correctness theorem (for refinements)\<close>
+corollary inline:
+  assumes "(inline c,s)\<Rightarrow>\<^bsup>z\<^esup> t"
+  obtains z' t'
+    where "(c,s) \<Rightarrow>'\<^bsup>z'\<^esup> t'"
+      and "t = t' on set (vars c)" 
+      and "z' \<le> z"
+  using inline_complete[where ?s'=s,OF assms] by auto
 
 end
